change of names, cleanup

src/definitions.lean
@@ -30,7 +30,6 @@ def bound (x : nat) : btree α → bool
 | (btree.node l k a r) :=
   x = k ∨ bound l ∨ bound r
 
--- swap nat / tree
 def forall_keys (p : nat → nat → Prop) : nat → btree α → Prop
 | x btree.empty := tt
 | x (btree.node l k a r) :=
@@ -52,7 +51,7 @@ def balanced : btree α → bool
   if height l ≥ height r then height l ≤ height r + 1
   else height r ≤ height l + 1
 
-def outLeft : btree α → bool
+def left_heavy : btree α → bool
 | btree.empty := ff
 | (btree.node l k a r) :=
   match l with
@@ -62,7 +61,7 @@ def outLeft : btree α → bool
     (height lr ≥ height r) ∧ (height r + 1 = height ll)
   end
 
-def outRight : btree α → bool
+def right_heavy : btree α → bool
 | btree.empty := ff
 | (btree.node l k a r) :=
   match r with
@@ -72,41 +71,41 @@ def outRight : btree α → bool
     (height rl ≤ height l) ∧ (height l + 1 = height rr)
   end
 
-def easyR : btree α → btree α
+def simple_right : btree α → btree α
 | btree.empty := btree.empty
 | (btree.node (btree.node ll lk la lr) k a r) := btree.node ll lk la (btree.node lr k a r)
 | (btree.node l k a r) := btree.node l k a r
 
-def easyL : btree α → btree α
+def simple_left : btree α → btree α
 | btree.empty := btree.empty
 | (btree.node l k a (btree.node rl rk ra rr)) := (btree.node (btree.node l k a rl) rk ra rr)
 | (btree.node l k a r) := btree.node l k a r
 
-def rotR : btree α → btree α
+def rotate_right : btree α → btree α
 | btree.empty := btree.empty
 | (btree.node l k a r) :=
   match l with
   | btree.empty := (btree.node l k a r)
   | (btree.node ll lk la lr) :=
-    if height ll < height lr then easyR (btree.node (easyL l) k a r)
-    else easyR (btree.node l k a r)
+    if height ll < height lr then simple_right (btree.node (simple_left l) k a r)
+    else simple_right (btree.node l k a r)
   end 
 
-def rotL : btree α → btree α
+def rotate_left : btree α → btree α
 | btree.empty := btree.empty
 | (btree.node l k a r) :=
   match r with
   | btree.empty := (btree.node l k a r)
   | (btree.node rl rk ra rr) :=
-    if height rr < height rl then easyL (btree.node l k a (easyR r))
-    else easyL (btree.node l k a r)
+    if height rr < height rl then simple_left (btree.node l k a (simple_right r))
+    else simple_left (btree.node l k a r)
   end
 
 def balance : btree α → btree α
 | btree.empty := btree.empty
 | (btree.node l k a r) :=
-  if outLeft (btree.node l k a r) then rotR (btree.node (balance l) k a r)
-  else if outRight (btree.node l k a r) then rotL (btree.node l k a (balance r))
+  if left_heavy (btree.node l k a r) then rotate_right (btree.node (balance l) k a r)
+  else if right_heavy (btree.node l k a r) then rotate_left (btree.node l k a (balance r))
   else btree.node l k a r
 
 def insert_balanced (x : nat) (v : α) : btree α → btree α
@@ -114,76 +113,75 @@ def insert_balanced (x : nat) (v : α) : btree α → btree α
 | (btree.node l k a r) :=
   if x < k then
     let nl := insert_balanced l in
-    if height nl > height r + 1 then rotR (btree.node nl k a r)
+    if height nl > height r + 1 then rotate_right (btree.node nl k a r)
     else btree.node nl k a r
   else if x > k then
     let nr := insert_balanced r in
-    if height nr > height l + 1 then rotL (btree.node l k a nr)
+    if height nr > height l + 1 then rotate_left (btree.node l k a nr)
     else btree.node l k a nr
   else btree.node l x v r
 
-def shrink : btree α → option (nat × α × btree α)
+def inorder_pred : btree α → option (nat × α × btree α)
 | btree.empty := none
 | (btree.node l k v r) := some $
-  match shrink r with
+  match inorder_pred r with
   | none := (k, v, l)
   | some (x, a, sh) :=
     if height l > height sh + 1
-      then (x, a, rotR (btree.node l k v sh))
+      then (x, a, rotate_right (btree.node l k v sh))
       else (x, a, btree.node l k v sh)
   end
 
-inductive shrink_view {α} : btree α → option (nat × α × btree α) → Sort*
-| empty : shrink_view empty none
-| nonempty_empty : ∀ {l k v r},
-  shrink r = none →
-  shrink_view (node l k v r) (some (k, v, l))
-| nonempty_nonempty₁ : ∀ {l k v r x a sh out},
-  shrink r = some (x, a, sh) →
-  height l > height sh + 1 →
-  out = some (x, a, rotR (btree.node l k v sh)) →
-  shrink_view (node l k v r) out
-| nonempty_nonempty₂ : ∀ {l k v r x a sh},
-  shrink r = some (x, a, sh) →
-  height l ≤ height sh + 1 →
-  shrink_view (node l k v r) (some (x, a, node l k v sh))
-
-def delRoot : btree α → btree α
+def del_node : btree α → btree α
 | btree.empty := btree.empty
 | (btree.node l k v r) :=
-  match shrink l with
+  match inorder_pred l with 
   | none := r
   | some (x, a, sh) :=
-    if height r > height sh + 1
-      then rotL (node sh x a r)
-      else node sh x a r
+    if height r > height sh + 1 then rotate_left (node sh x a r)
+    else node sh x a r
   end
 
-/- delRoot_view t dt ↔ delRoot t = dt -/
-inductive delRoot_view {α} : btree α → btree α → Sort*
-| empty : delRoot_view empty empty
+inductive inorder_pred_view {α} : btree α → option (nat × α × btree α) → Sort*
+| empty : inorder_pred_view empty none
 | nonempty_empty : ∀ {l k v r},
-  shrink l = none →
-  delRoot_view (node l k v r) r
-| nonempty_nonempty₁ : ∀ {l k v r x a sh},
-  shrink l = some (x, a, sh) →
-  height r > height sh + 1 →
-  delRoot_view (node l k v r) (rotL (node sh x a r))
+  inorder_pred r = none →
+  inorder_pred_view (node l k v r) (some (k, v, l))
+| nonempty_nonempty₁ : ∀ {l k v r x a sh out},
+  inorder_pred r = some (x, a, sh) →
+  height l > height sh + 1 →
+  out = some (x, a, rotate_right (btree.node l k v sh)) →
+  inorder_pred_view (node l k v r) out
 | nonempty_nonempty₂ : ∀ {l k v r x a sh},
-  shrink l = some (x, a, sh) →
+  inorder_pred r = some (x, a, sh) →
+  height l ≤ height sh + 1 →
+  inorder_pred_view (node l k v r) (some (x, a, node l k v sh))
+
+/- delRoot_view t dt ↔ delRoot t = dt -/
+inductive del_node_view {α} : btree α → btree α → Sort*
+| empty : del_node_view empty empty
+| nonempty_empty : ∀ {l k v r},
+  inorder_pred l = none →
+  del_node_view (node l k v r) r
+| nonempty_nonempty₁ : ∀ {l k v r x a sh},
+  inorder_pred l = some (x, a, sh) →
+  height r > height sh + 1 →
+  del_node_view (node l k v r) (rotate_left (node sh x a r))
+| nonempty_nonempty₂ : ∀ {l k v r x a sh},
+  inorder_pred l = some (x, a, sh) →
   height r ≤ height sh + 1 →
-  delRoot_view (node l k v r) (node sh x a r)
+  del_node_view (node l k v r) (node sh x a r)
 
 def delete (x : nat) : btree α → btree α
 | btree.empty := btree.empty
 | (btree.node l k a r) :=
   let dl := delete l in
   let dr := delete r in
-  if x = k then delRoot (btree.node l k a r)
+  if x = k then del_node (btree.node l k a r)
   else if x < k then
-    if height r > height dl + 1 then rotL (btree.node dl k a r)
+    if height r > height dl + 1 then rotate_left (btree.node dl k a r)
     else btree.node dl k a r
-  else if height l > height dr + 1 then rotR (btree.node l k a dr)
+  else if height l > height dr + 1 then rotate_right (btree.node l k a dr)
   else (btree.node l k a dr)
 
 end btree
