src/deletion.lean
@@ -1,4 +1,4 @@
-import basic
+import definitions
 import rotations
 import tactic.linarith
 import tactic.induction
@@ -12,72 +12,72 @@ open rotation_lemmas
 
 variables {α : Type u}
 
-lemma delRoot_delRoot_view (t : btree α) :
-  delRoot_view t (delRoot t) :=
+lemma del_node_del_node_view (t : btree α) :
+  del_node_view t (del_node t) :=
 begin
   cases t,
   case empty {
-    exact delRoot_view.empty,
+    exact del_node_view.empty,
   },
   case node : l k a r {
-    dsimp [delRoot],
-    cases h : shrink l,
+    dsimp [del_node],
+    cases h : inorder_pred l,
     case none {
-      dsimp [delRoot._match_1],
-      apply delRoot_view.nonempty_empty; assumption,
+      dsimp [del_node._match_1],
+      apply del_node_view.nonempty_empty; assumption,
     },
     case some {
       rcases val with ⟨x, a', sh⟩,
-      dsimp only [delRoot._match_1],
+      dsimp only [del_node._match_1],
       by_cases h' : height r > height sh + 1,
       { simp only [if_pos h'],
-        apply delRoot_view.nonempty_nonempty₁; assumption,
+        apply del_node_view.nonempty_nonempty₁; assumption,
       },
       { simp only [if_neg h'],
-        apply delRoot_view.nonempty_nonempty₂; try { assumption, },
+        apply del_node_view.nonempty_nonempty₂; try { assumption, },
         linarith,
       },
     },
   },
 end
 
-lemma shrink_shrink_view (t : btree α) : 
-  shrink_view t (shrink t) :=
+lemma inorder_pred_inorder_pred_view (t : btree α) : 
+  inorder_pred_view t (inorder_pred t) :=
 begin
  cases t,
  case empty {
-  exact shrink_view.empty,
+  exact inorder_pred_view.empty,
  },
  case node : l k a r {
-  dsimp [shrink],
-  cases h : shrink r,
+  dsimp [inorder_pred],
+  cases h : inorder_pred r,
   case none {
-    dsimp only [shrink._match_1],
-    apply shrink_view.nonempty_empty; assumption,
+    dsimp only [inorder_pred._match_1],
+    apply inorder_pred_view.nonempty_empty; assumption,
   },
   case some {
     rcases val with ⟨x, a', sh⟩,
-    dsimp only [shrink._match_1],
+    dsimp only [inorder_pred._match_1],
     by_cases h' : (height l > height sh + 1),
     { simp only [if_pos h'], 
-      apply shrink_view.nonempty_nonempty₁, try { assumption },
+      apply inorder_pred_view.nonempty_nonempty₁, try { assumption },
       assumption, simp,
     },
     { simp only [if_neg h'],
-      apply shrink_view.nonempty_nonempty₂, try { assumption },
+      apply inorder_pred_view.nonempty_nonempty₂, try { assumption },
       linarith,
     },
   },
  },
 end
 
-lemma shrink_ordered (l r sh : btree α) (k x : nat) (v a : α) :
-  ordered (btree.node l k v r) ∧ shrink (btree.node l k v r) = some (x, a, sh) → (ordered sh ∧ forall_keys (>) x sh) :=
+lemma inorder_pred_ordered (l r sh : btree α) (k x : nat) (v a : α) :
+  ordered (btree.node l k v r) ∧ inorder_pred (btree.node l k v r) = some (x, a, sh) → (ordered sh ∧ forall_keys (>) x sh) :=
 begin
   intro h₁,
   induction r generalizing x a sh l k v,
   case empty {
-    simp [ordered, shrink] at h₁,
+    simp [ordered, inorder_pred] at h₁,
     cases_matching* (_ ∧ _),
     rw ← h₁_right_right_right,
     split,
@@ -86,7 +86,7 @@ begin
   },
   case node : rl rk ra rr ihl ihr {
     cases_matching* (_ ∧ _),
-    cases' shrink_shrink_view (node l k v (node rl rk ra rr)),
+    cases' inorder_pred_inorder_pred_view (node l k v (node rl rk ra rr)),
     case nonempty_empty { cases' h₁_right, 
       simp [ordered] at h₁_left,
       finish,
@@ -95,7 +95,7 @@ begin
       cases' h₁_right,
       clear h_2,
       split,
-      { apply rotR_ordered, 
+      { apply rotate_right_ordered, 
         rw ordered at *,
         { specialize ihr x_1 a_1 sh_1 rl rk ra, 
           have h : ordered (node rl rk ra rr),
@@ -116,20 +116,20 @@ begin
   },
 end
 
-lemma delRoot_ordered (t : btree α) :
-  ordered t → ordered (delRoot t) :=
+lemma del_node_ordered (t : btree α) :
+  ordered t → ordered (del_node t) :=
 begin
   intro h₁,
   cases t,
   case empty {
-    simp [delRoot, ordered],
+    simp [del_node, ordered],
   },
   case node : tl tk ta tr {
-    cases' delRoot_delRoot_view (node tl tk ta tr),
+    cases' del_node_del_node_view (node tl tk ta tr),
     { simp only [ordered] at h₁, 
       apply and.left (and.right h₁),
     },
-    { apply rotL_ordered,
+    { apply rotate_left_ordered,
       rw ordered,
       sorry,
     },
@@ -149,7 +149,7 @@ begin
     simp only [delete],
     by_cases c₁ : (k = tk),
     { simp only [if_pos c₁], 
-      apply delRoot_ordered,
+      apply del_node_ordered,
       exact h₁,
     },
     { simp only [if_neg c₁],
@@ -157,7 +157,7 @@ begin
       { simp only [if_pos c₂], 
         by_cases c₃ : (height (delete k tl) + 1 < height tr),
         { simp only [if_pos c₃],
-          apply rotL_ordered,
+          apply rotate_left_ordered,
           rw ordered at *,
           cases_matching* (_ ∧ _),
           repeat { split }; try { assumption },
@@ -175,7 +175,7 @@ begin
       { simp only [if_neg c₂], 
         by_cases c₃ : (height tl > height (delete k tr) + 1),
         { simp only [if_pos c₃], 
-          apply rotR_ordered,
+          apply rotate_right_ordered,
           rw ordered at *,
           cases_matching* (_ ∧ _),
           repeat { split }; try { assumption },
@@ -213,7 +213,7 @@ begin
       { simp only [if_pos c₂], 
         by_cases c₃ : (height tr > height (delete k tl) + 1),
         { simp only [if_pos c₃], 
-          apply rotL_keys,
+          apply rotate_left_keys,
           simp [bound] at *,
           cases_matching* (_ ∧ _),
           repeat { split }; try { assumption },
@@ -228,7 +228,7 @@ begin
       { simp only [if_neg c₂], 
         by_cases c₃ : (height tl > height (delete k tr) + 1),
         { simp only [if_pos c₃], 
-          apply rotR_keys,
+          apply rotate_right_keys,
           simp [bound] at *,
           cases_matching* (_ ∧ _),
           repeat { split }; try { assumption },
